### Exercise 1.13

Prove that $Fib(n)$ is the closest to

Let

$$
g(n) = \frac{\phi^{n}}{\sqrt{5}}
h(n) = \frac{\phi^{n} - \psi^{n}}{\sqrt{5}}
$$

First, we prove by induction that Fib(n) = h(n).

For $n = 0$:

$$
\begin{align}
Fib(0) & = 0, \text{(by definition)} \\
h(0) & = \frac{\phi^{0} - \psi^{0}}{\sqrt{5}} \\
     & = \frac{1 - 1}{0} = 0
\end{align}
$$

For $n = 1$:

$$
\begin{align}
Fib(1) & = 1, \text{(by definition)} \\
h(1) & = \frac{\phi^{1} - \psi^{1}}{\sqrt{5}} \\
     & = \frac{\frac{1 + \sqrt{5}}{2} - \frac{1 - \sqrt{5}}{2}}{\sqrt{5}} \\
     & = \frac{1 + \sqrt{5} - 1 + \sqrt{5}}{2 \sqrt{5}} \\
     & = \frac{2 \sqrt{5}}{2 \sqrt{5}} \\
     & = 1
\end{align}
$$

Inductive step:

$$
Fib(k+2) = Fib(k+1) + Fib(k)
$$

We need to show that:

```
a <- bq + aq + ap = a'
b <- bp + aq = b'
```

and

```
a' <- b'q + a'q + a'p = a''
b' <- b'p + a'q = b''
```

Performing substitution:

```
a' <- (bp + aq)q + (bq + aq + ap)q + (bq + aq + ap)p
   <- aq^2 + bpq + bq^2 + aq^2 + apq + bpq + apq + ap^2
   <- 2aq^2 + 2bpq + 2apq + ap^2 + bq^2
   <- 2(aq^2 + bpq + apq) + ap^2 + bq^2
   <- (2a+b)q^2 + (a)p^2 + 2(a+b)pq
   <- (2q^2 + p^2 + 2pq)a + (q^2 + 2pq)b
   <- (q^2 + 2pq)a + (p^2 + q^2)a + (q^2 + 2pq)b
   <- (q' + p')a + (q')b
   <- (q')a + (p')a + (q')b
```

```
b' <- (bp + aq)p + (bq + aq + ap)q
   <- bp^2 + apq + bq^2 + aq^2 + apq
   <- (b)p^2 + (a+b)q^2 + (2a)pq
   <- (q^2 + 2pq)a + (p^2 + q^2)b
   <- (q')a + (p')b
```
